Isabelle_Set/Examples/Typing_Examples.thy
@@ -3,7 +3,7 @@ theory Typing_Examples
 begin
 
 lemma empty_type[type]: "{} : subset A"
-  unfolding element_typedef by auto
+  by stauto
 
 text \<open>
   The following typing rules are less general than what could be proved, since the \<open>bool\<close> soft
@@ -14,10 +14,10 @@ text \<open>
   type inference algorithm.
 \<close>
 lemma All_type[type]: "HOL.All : ((A::set type) \<Rightarrow> any) \<Rightarrow> any"
-  by (intro Pi_typeI any_TypeI)
+  by (intro Pi_typeI any_typeI)
 
 lemma mem_type[type]: "(\<in>) : element A \<Rightarrow> subset A \<Rightarrow> any"
-  by (intro Pi_typeI any_TypeI)
+  by (intro Pi_typeI any_typeI)
 
 lemma Cons_type[type]: "Set_Theory.Cons : element A \<Rightarrow> subset A \<Rightarrow> subset A"
   by (intro Pi_typeI, unfold element_type_iff Pow_rule) auto
@@ -26,10 +26,10 @@ lemma Cons_type[type]: "Set_Theory.Cons : element A \<Rightarrow> subset A \<Rig
 text \<open>The following statements are also provable, but not helpful:\<close>
 
 lemma "HOL.All : (Type1 \<Rightarrow> Type2) \<Rightarrow> any"
-  by (intro Pi_typeI any_TypeI)
+  by (intro Pi_typeI any_typeI)
 
 lemma "(\<in>) : Type1 \<Rightarrow> Type2 \<Rightarrow> any"
-  by (intro Pi_typeI any_TypeI)
+  by (intro Pi_typeI any_typeI)
 
 
 
